Refactor

FormalizationOfComputability/Phi.lean
@@ -12,7 +12,7 @@ This file contains the definitions most commonly used by working computability t
 the use functions ϕₑ, the enumerable sets Wₑ, and their computable
 approximations ϕ_{e, s} and W_{e, s}.
 
-In some sense Phi_s and Phi are merely wrappers for evaln and eval, respectively,
+In some sense ϕ_s and ϕ are merely wrappers for evaln and eval, respectively,
 modified to match common computability theory notation.
 
 ## Main results
@@ -79,74 +79,86 @@ private lemma helperlemma (x : ℕ) : Option.none = some x → False := by
     intro h
     simp_all only [reduceCtorEq]
 
+variable {e s t n x y : ℕ} {X : Set ℕ}
+
+
 /- ϕₑ,ₛ(n), the eth Turing program evaluated for s steps on input n.
 Following Soare, we require the index, input, and output to be less than s -/
-def Phi_s (e s n : ℕ) : Option ℕ :=
+def ϕ_s (e s n : ℕ) : Option ℕ :=
     if (e < s) ∧ (∃ y < s, y ∈ evaln s (ofNatCode e) n)
     then evaln s (ofNatCode e) n
     else Option.none
 
 /- ϕₑ(n), the eth Turing program evaluated on input n -/
-def Phi (e : ℕ) : ℕ →. ℕ := eval (ofNatCode e)
-
-/- ϕₑ,ₛ(n) is decidable -/
-instance (e s n : ℕ) : Decidable (Phi_s e s n).isSome :=
-  (if e < s ∧ ∃ y < s, evaln s (ofNatCode e) n = some y then evaln s (ofNatCode e) n
-    else Option.none).isSome.decEq true
+def ϕ (e : ℕ) : ℕ →. ℕ := eval (ofNatCode e)
 
 /- ϕₑ,ₛ(n)↓ iff it has an output -/
 @[grind, simp]
-def Phi_s_halts (e s n : ℕ) : Prop := (Phi_s e s n).isSome
+def ϕ_s_halts (e s n : ℕ) : Prop := (ϕ_s e s n).isSome
 
 /- ϕₑ(n)↓ iff it has an output -/
 @[grind, simp]
-def Phi_halts (e n : ℕ) : Prop := (Phi e n).Dom
+def ϕ_halts (e n : ℕ) : Prop := (ϕ e n).Dom
 
-/- ϕₑ,ₛ(n) is decidable -/
-instance (e s n : ℕ) : Decidable (Phi_s_halts e s n) :=
-  instDecidableEqBoolIsSomeNatPhi_sTrue e s n
+/- If ϕₑ,ₛ(n)↓, then ϕₑ(n)↓ -/
+lemma ϕ_sound (h : ϕ_s_halts e s n) : ϕ_halts e n := by
+  have h1 : ∃ s, ϕ_s_halts e s n := by exact ⟨s, h⟩
+  revert h1
+  unfold ϕ_s_halts ϕ_s
+  unfold ϕ_halts ϕ
+  simp only [Part.dom_iff_mem, evaln_complete]
+  grind
 
-/- Wₑ,ₛ = the domain of ϕₑ,ₛ. As all inputs n ≥ s do not halt, this set is necessarily finite. -/
-@[grind, simp]
-def W_s (e s : ℕ): Finset ℕ := (Finset.range s).filter (Phi_s_halts e s)
-
-/- Wₑ = {n | ϕₑ(n)↓} -/
-@[grind, simp]
-def W (e : ℕ) : Set ℕ := (Phi e).Dom
-
-instance (e s n : ℕ) : Decidable (n ∈ W_s e s) :=
-  Finset.decidableMem n (Finset.filter (Phi_s_halts e s) (Finset.range s))
-
-variable {e s t n x y : ℕ} {X : Set ℕ}
+/- ϕₑ(n)↓ iff there is a stage s at which ϕₑ,ₛ(n)↓ -/
+@[grind =, simp]
+lemma ϕ_complete : ϕ_halts e n ↔ ∃ s, ϕ_s_halts e s n := by
+  constructor
+  · unfold ϕ_s_halts ϕ_halts ϕ_s ϕ
+    simp only [Part.dom_iff_mem, evaln_complete, Option.mem_def, Option.isSome_iff_exists,
+    Option.ite_none_right_eq_some, exists_and_left]
+    intro ⟨x, ⟨k, h⟩⟩
+    let N := e + x + k + 1 -- one plus the maximum of e, x, and k would also work
+    have he : e < N := by omega
+    have hx : x < N := by omega
+    have hk : k < N := by omega
+    use N
+    simp only [he, true_and]
+    refine exists_and_exists_comm.mpr ?_
+    use x
+    use x
+    simp only [hx, true_and, and_self]
+    exact evaln_mono (le_of_succ_le hk) h
+  · intro ⟨s, h⟩
+    exact ϕ_sound h
 
 /- If ϕₑ,ₛ(n)↓, then n < s -/
 @[grind →, simp]
-lemma halt_input_bound (h : Phi_s_halts e s n) : n < s := by
-  simp only [Phi_s_halts, Phi_s, Option.mem_def, Option.isSome_iff_exists,
+lemma ϕ_input_bound (h : ϕ_s_halts e s n) : n < s := by
+  simp only [ϕ_s_halts, ϕ_s, Option.mem_def, Option.isSome_iff_exists,
     Option.ite_none_right_eq_some, exists_and_left] at h
   obtain ⟨x, hx⟩ := h.right
   exact Code.evaln_bound hx
 
 /- If ϕₑ,ₛ(n) = y, then y < s -/
 @[grind →, simp]
-lemma halt_output_bound (h : y ∈ (Phi_s e s n)) : y < s := by
-  simp only [Phi_s, Option.mem_def, Option.ite_none_right_eq_some] at h
+lemma ϕ_output_bound (h : y ∈ (ϕ_s e s n)) : y < s := by
+  simp only [ϕ_s, Option.mem_def, Option.ite_none_right_eq_some] at h
   grind
 
 /- If ϕₑ,ₛ(n)↓, then e < s -/
 @[grind →, simp]
-lemma halt_index_bound (h : Phi_s_halts e s n) : e < s := by grind [Phi_s_halts, Phi_s]
+lemma ϕ_index_bound (h : ϕ_s_halts e s n) : e < s := by grind [ϕ_s_halts, ϕ_s]
 
 /- Helper lemmas - ϕ_{e, 0}(n)↑ -/
 @[grind →, simp]
-lemma halt_stage_gt_zero (h : Phi_s_halts e s n) : s > 0 := by grind [Phi_s_halts, Phi_s]
+lemma halt_stage_gt_zero (h : ϕ_s_halts e s n) : s > 0 := by grind [ϕ_s_halts, ϕ_s]
 
 @[grind ., simp]
-lemma stage_zero_diverges : ¬ Phi_s_halts e 0 n := by grind [Phi_s_halts, Phi_s]
+lemma stage_zero_diverges : ¬ ϕ_s_halts e 0 n := by grind [ϕ_s_halts, ϕ_s]
 
 open Primrec
 
--- a helper lemma for showing that phi_s is primitive recursive
+-- a helper lemma for showing that ϕ_s is primitive recursive
 private lemma bounded_exists (f : ℕ → ℕ → Prop) (s : ℕ) [DecidableRel f]
     (hf : PrimrecRel f) :
       PrimrecPred (λ n => ∃ y < s, (f y n)) := by
@@ -158,73 +170,46 @@ private lemma bounded_exists (f : ℕ → ℕ → Prop) (s : ℕ) [DecidableRel 
     simp_all only [List.mem_range]
 
 /- ϕₑ,ₛ is a primitive recursive function -/
--- couldn't I do this by knowing that Phi_s is decidable? Or vice versa?
-lemma phi_s_primrec : Primrec (Phi_s e s) := by
+lemma ϕ_s_primrec : Primrec (ϕ_s e s) := by
   have h := primrec_evaln.comp (pair (pair (const s) (const (ofNatCode e))) .id)
   apply ite (PrimrecPred.and (PrimrecRel.comp nat_lt (const e) (const s)) ?_) h (const Option.none)
   apply bounded_exists
   simp only [PrimrecRel, Option.mem_def]
   exact PrimrecRel.comp Primrec.eq (.comp h snd) (option_some_iff.mpr fst)
 
-lemma phi_s_halts_primrec : PrimrecPred (Phi_s_halts e s) := by
-  have h (n : ℕ) : (∃ x, Phi_s e s n = some x) ↔ (∃ x < s, Phi_s e s n = some x) := by
+/- ϕ_s_halts is a primitive recursive predicate -/
+lemma ϕ_s_halts_primrec : PrimrecPred (ϕ_s_halts e s) := by
+  have h (n : ℕ) : (∃ x, ϕ_s e s n = some x) ↔ (∃ x < s, ϕ_s e s n = some x) := by
     constructor
     · intro ⟨x, h⟩
       use x
-      simp only [halt_output_bound h, h, and_self]
+      simp only [ϕ_output_bound h, h, and_self]
     · simp_all
-  unfold Phi_s_halts
+  unfold ϕ_s_halts
   simp only [Option.isSome_iff_exists, h]
   apply bounded_exists
-  apply PrimrecRel.comp₂ Primrec.eq (comp₂ (phi_s_primrec) (Primrec₂.right))
+  apply PrimrecRel.comp₂ Primrec.eq (comp₂ (ϕ_s_primrec) (Primrec₂.right))
   exact comp₂ option_some Primrec₂.left
 
+/- ϕₑ,ₛ(n) is decidable -/
+instance (e s n : ℕ) : Decidable (ϕ_s e s n).isSome :=
+  (ϕ_s e s n).isSome.decEq true
+
+/- ϕₑ,ₛ(n) is decidable -/
+instance (e s n : ℕ) : Decidable (ϕ_s_halts e s n) :=
+  instDecidableEqBoolIsSomeNatϕ_sTrue e s n
+
 /- ϕₑ is a partial computable function -/
-theorem phi_partrec : Nat.Partrec (Phi e) := by
-  unfold Phi
+theorem ϕ_partrec : Nat.Partrec (ϕ e) := by
+  unfold ϕ
   rw [Code.exists_code]
   use ofNatCode e
 
-/- The Wₑ,ₛ are primitive recursive-/
-lemma W_s_Primrec : Primrec.set (W_s e s) := by
-  simp only [Primrec.set, W_s, Finset.coe_filter, Finset.mem_range, Set.mem_setOf_eq]
-  use Phi_s_halts e s
-  constructor
-  · exact Primrec.ite (phi_s_halts_primrec) (const true) (const false)
-  · grind
-
-/- The Wₑ are Σ01 -/
-lemma W_Sigma01 (e : ℕ) : Sigma01 (W e) := by
-  use λ n ↦ (Phi e n).map (λ _ => ())
-  constructor
-  · refine Partrec.map ?_ (Primrec₂.to_comp (Primrec₂.const ()))
-    constructor
-    · exact phi_partrec
-    · exact Partrec.nat_iff.mp (Computable.partrec Computable.id)
-  · rfl
-
-/- Sigma01 sets can be written as Wₑ -/
-lemma Sigma01_is_W (h : Sigma01 X) : ∃ e, X = W e := by
-· obtain ⟨f, ⟨h1, h2⟩⟩ := h
-  let f_nat : ℕ →. ℕ := λ n => (f n).map (λ _ => 1)
-  have h3 := Partrec.nat_iff.mp (Partrec.map h1 (Primrec₂.to_comp (Primrec₂.const 1)))
-  have h4 : f.Dom = f_nat.Dom := rfl
-  rw [Code.exists_code] at h3
-  obtain ⟨c, h3⟩ := h3
-  rw [← h2, h4]
-  use c.encodeCode
-  unfold W Phi
-  rw [← ofNatCode_encode c]
-  exact congrArg PFun.Dom (id (Eq.symm h3))
-
-/- The Σ01 sets are exactly the Wₑ -/
-lemma Sigma01_iff_W : Sigma01 X ↔ ∃ e, X = W e := by grind [Sigma01_is_W, W_Sigma01]
-
 /- Monotonicity of halting: if s < t and ϕ_{e,s}(n)↓, then ϕ_{e,t}(n)↓ -/
 @[grind →, simp]
-lemma phi_halts_mono (h : s ≤ t) (h1 : Phi_s_halts e s n) : Phi_s_halts e t n := by
+lemma ϕ_halts_mono (h : s ≤ t) (h1 : ϕ_s_halts e s n) : ϕ_s_halts e t n := by
   revert h1
-  simp only [Phi_s_halts, Phi_s, Option.mem_def, Option.isSome_iff_exists,
+  simp only [ϕ_s_halts, ϕ_s, Option.mem_def, Option.isSome_iff_exists,
     Option.ite_none_right_eq_some, exists_and_left, and_imp, forall_exists_index]
   intro _ x _ h3 _ _
   constructor
@@ -238,53 +223,29 @@ lemma phi_halts_mono (h : s ≤ t) (h1 : Phi_s_halts e s n) : Phi_s_halts e t n 
 
 /- Reverse monotonicity of halting: if s < t and ϕ_{e,t}(n)↑, then ϕ_{e,s}(n)↑ -/
 @[grind →, simp]
-lemma phi_halts_mono_reverse (h : s ≤ t) (h1 : ¬ Phi_s_halts e t n) : ¬ Phi_s_halts e s n := by
+lemma ϕ_halts_mono_reverse (h : s ≤ t) (h1 : ¬ ϕ_s_halts e t n) : ¬ ϕ_s_halts e s n := by
   grind
 
 /- The least stage s at which ϕₑ,ₛ(n)↓ (if it exists) -/
 @[grind, simp]
-def runtime (e n : ℕ) : Part ℕ := rfind (fun s => (Phi_s e s n).isSome)
+def runtime (e n : ℕ) : Part ℕ := rfind (fun s => (ϕ_s e s n).isSome)
 
 /- TODO: runtime lemmas can be cleaned up with Nat.rfind spec/min? -/
 /- Runtime r is minimal - if s < r, then ϕₑ,ₛ(n)↑ -/
 @[simp]
-lemma runtime_spec (r : ℕ) (h : r ∈ runtime e n) : Phi_s_halts e r n := by
+lemma runtime_spec (r : ℕ) (h : r ∈ runtime e n) : ϕ_s_halts e r n := by
   simp_all only [runtime, Part.coe_some, mem_rfind, Part.mem_some_iff, Bool.true_eq, Bool.false_eq,
-  Option.isSome_eq_false_iff, Option.isNone_iff_eq_none, Phi_s_halts]
+  Option.isSome_eq_false_iff, Option.isNone_iff_eq_none, ϕ_s_halts]
 
-lemma runtime_min (r : ℕ) (h : r ∈ (runtime e n)) : ∀ t, t < r → ¬ Phi_s_halts e t n := by
+lemma runtime_min (r : ℕ) (h : r ∈ (runtime e n)) : ∀ t, t < r → ¬ ϕ_s_halts e t n := by
   simp_all
-
-/- ϕₑ(n)↓ iff there is a stage s at which ϕₑ,ₛ(n)↓ -/
-@[grind =, simp]
-lemma phi_halts_stage_exists : Phi_halts e n ↔ ∃ s, Phi_s_halts e s n := by
-  unfold Phi_s_halts Phi_halts Phi_s Phi
-  simp only [Part.dom_iff_mem, evaln_complete, Option.mem_def, Option.isSome_iff_exists,
-    Option.ite_none_right_eq_some, exists_and_left]
-  constructor
-  · intro ⟨x, ⟨k, h⟩⟩
-    use e+x+k+1 -- one plus the maximum of e, x, and k would also work
-    constructor
-    · constructor
-      · linarith -- e < e+x+k+1
-      · use x
-        constructor
-        · linarith -- x < e+x+k+1
-        · apply evaln_mono
-          · linarith
-          · exact h
-    · use x
-      apply evaln_mono
-      · linarith -- k < e+x+k+1
-      · exact h
-  · grind
 
 /- ϕₑ(n)↓ iff there is a *least* stage s at which ϕₑ,ₛ(n)↓ -/
 @[grind =, simp]
-lemma phi_halts_runtime_exists : Phi_halts e n ↔ ∃ r, r ∈ runtime e n := by
+lemma ϕ_halts_runtime_exists : ϕ_halts e n ↔ ∃ r, r ∈ runtime e n := by
   constructor
   · intro h
-    rcases (phi_halts_stage_exists.mp h) with ⟨s, hs⟩
+    rcases (ϕ_complete.mp h) with ⟨s, hs⟩
     have h1 : (runtime e n).Dom := by
       unfold runtime
       use s
@@ -293,15 +254,61 @@ lemma phi_halts_runtime_exists : Phi_halts e n ↔ ∃ r, r ∈ runtime e n := b
       exact hs
     simpa [Part.dom_iff_mem] using h1
   · intro ⟨r, h⟩
-    apply phi_halts_stage_exists.mpr
+    apply ϕ_complete.mpr
     apply runtime_spec at h
     exact ⟨r, h⟩
 
+/- Wₑ,ₛ = the domain of ϕₑ,ₛ. As all inputs n ≥ s do not halt, this set is necessarily finite. -/
+@[grind, simp]
+def W_s (e s : ℕ): Finset ℕ := (Finset.range s).filter (ϕ_s_halts e s)
+
+/- Wₑ = {n | ϕₑ(n)↓} -/
+@[grind, simp]
+def W (e : ℕ) : Set ℕ := (ϕ e).Dom
+
+instance (e s n : ℕ) : Decidable (n ∈ W_s e s) :=
+  Finset.decidableMem n (Finset.filter (ϕ_s_halts e s) (Finset.range s))
+
+/- The Wₑ,ₛ are primitive recursive-/
+lemma W_s_Primrec : Primrec.set (W_s e s) := by
+  simp only [Primrec.set, W_s, Finset.coe_filter, Finset.mem_range, Set.mem_setOf_eq]
+  use ϕ_s_halts e s
+  constructor
+  · exact Primrec.ite (ϕ_s_halts_primrec) (const true) (const false)
+  · grind
+
+/- The Wₑ are Σ01 -/
+lemma W_Sigma01 (e : ℕ) : Sigma01 (W e) := by
+  use λ n ↦ (ϕ e n).map (λ _ => ())
+  constructor
+  · refine Partrec.map ?_ (Primrec₂.to_comp (Primrec₂.const ()))
+    constructor
+    · exact ϕ_partrec
+    · exact Partrec.nat_iff.mp (Computable.partrec Computable.id)
+  · rfl
+
+/- Sigma01 sets can be written as Wₑ -/
+lemma Sigma01_is_W (h : Sigma01 X) : ∃ e, X = W e := by
+· obtain ⟨f, ⟨h1, h2⟩⟩ := h
+  let f_nat : ℕ →. ℕ := λ n => (f n).map (λ _ => 1)
+  have h3 := Partrec.nat_iff.mp (Partrec.map h1 (Primrec₂.to_comp (Primrec₂.const 1)))
+  have h4 : f.Dom = f_nat.Dom := rfl
+  rw [Code.exists_code] at h3
+  obtain ⟨c, h3⟩ := h3
+  rw [← h2, h4]
+  use c.encodeCode
+  unfold W ϕ
+  rw [← ofNatCode_encode c]
+  exact congrArg PFun.Dom (id (Eq.symm h3))
+
+/- The Σ01 sets are exactly the Wₑ -/
+lemma Sigma01_iff_W : Sigma01 X ↔ ∃ e, X = W e := by grind [Sigma01_is_W, W_Sigma01]
+
 /- ϕₑ,ₛ(n)↓ iff n ∈ Wₑ,ₛ -/
 @[simp]
-lemma W_s_Phi_s : n ∈ W_s e s ↔ Phi_s_halts e s n := by
-  simp_all only [W_s, Finset.mem_filter, Finset.mem_range, Phi_s_halts, and_iff_right_iff_imp]
-  exact fun a ↦ halt_input_bound a
+lemma W_s_ϕ_s : n ∈ W_s e s ↔ ϕ_s_halts e s n := by
+  simp_all only [W_s, Finset.mem_filter, Finset.mem_range, ϕ_s_halts, and_iff_right_iff_imp]
+  exact fun a ↦ ϕ_input_bound a
 
 @[simp]
 lemma Ws_gt_zero : n ∈ W_s e s → s > 0 := by grind
@@ -311,7 +318,7 @@ lemma Ws_zero_empty : W_s e 0 = ∅ := by grind
 
 /- ϕₑ(x)↓ ↔ x ∈ Wₑ -/
 @[simp]
-lemma mem_W_phi : n ∈ W e ↔ Phi_halts e n := by exact Eq.to_iff rfl
+lemma mem_W_ϕ : n ∈ W e ↔ ϕ_halts e n := by exact Eq.to_iff rfl
 
 /- Monotonicity of W_s: W_s ⊆ W_{e, s+1}  -/
 @[simp]
@@ -324,8 +331,8 @@ lemma W_s_mono_reverse (h : s ≤ t) (hx : x ∉ W_s e t) : x ∉ W_s e s := by 
 /- Membership in some W_{e,s} implies runtime r exists, and membership in W_{e, r}-/
 @[grind ., simp]
 lemma Ws_runtime (h : n ∈ W_s e s) : ∃ r, r ∈ runtime e n ∧ n ∈ W_s e r := by
-  have ⟨r, h1⟩ := phi_halts_runtime_exists.mp (phi_halts_stage_exists.mpr ⟨s, W_s_Phi_s.mp h⟩)
-  refine ⟨r, ⟨h1, W_s_Phi_s.mpr ?_⟩⟩
+  have ⟨r, h1⟩ := ϕ_halts_runtime_exists.mp (ϕ_complete.mpr ⟨s, W_s_ϕ_s.mp h⟩)
+  refine ⟨r, ⟨h1, W_s_ϕ_s.mpr ?_⟩⟩
   apply runtime_spec at h1
   exact h1
 
@@ -333,9 +340,9 @@ lemma Ws_runtime (h : n ∈ W_s e s) : ∃ r, r ∈ runtime e n ∧ n ∈ W_s e 
 @[grind! ., simp]
 lemma W_s_subset_W : ↑(W_s e s) ⊆ W e := by
   intro x h
-  rw [mem_W_phi]
+  rw [mem_W_ϕ]
   simp only [W_s, Finset.coe_filter, Finset.mem_range, Set.mem_setOf_eq] at h
-  rw [phi_halts_stage_exists]
+  rw [ϕ_complete]
   grind
 
 /- Wₑ = ⋃ₛ Wₑ,ₛ -/
@@ -343,8 +350,8 @@ lemma W_s_subset_W : ↑(W_s e s) ⊆ W e := by
 lemma W_mem_iff_W_s : n ∈ W e ↔ ∃ s, n ∈ W_s e s := by
   constructor
   · intro h
-    simp only [W_s_Phi_s]
-    exact phi_halts_stage_exists.mp (mem_W_phi.mp h)
+    simp only [W_s_ϕ_s]
+    exact ϕ_complete.mp (mem_W_ϕ.mp h)
   · grind
 
 lemma W_eq_union_W_s : W e = ⋃ (s : ℕ), W_s e s := by
